Made Decode.v in MIPSmodel work.

MIPSmodel/Decode.v
@@ -11,95 +11,83 @@
 
 (* This file provides simple bit-level parsing combinators for disassembling
  * MIPS 32-bit binaries. *)
-Require Coqlib.
 Require Import Coq.Init.Logic.
 Require Import Bool.
 Require Import List.
 Require Import String.
-Require Import Maps.
 Require Import Ascii.
 Require Import ZArith.
 Require Import Eqdep.
-Require Import Parser.
+
+Require Import Shared.Coqlib.
+Require Import Shared.Maps.
+
 Unset Automatic Introduction.
 Set Implicit Arguments.
 Local Open Scope Z_scope.
 
 
-Require ExtrOcamlString.
-Require ExtrOcamlNatBigInt.
+(* Module MIPS_PARSER. *)
+(*   Module MIPS_BASE_PARSER := Parser.Parser(MIPS_PARSER_ARG). *)
+  (* Import MIPS_BASE_PARSER. *)
 
-
-(* a module for generating the parser for x86 instructions *)
-Module MIPS_PARSER_ARG.
   Require Import MIPSSyntax.
-  Require Import Bits.
-  
-  Definition char_p : Set := bool.
-  Definition char_eq : forall (c1 c2:char_p), {c1=c2}+{c1<>c2} := bool_dec.
-  Inductive type : Set := 
-  | Int_t : type
-  | Register_t : type
-  | Shamt5_t : type
-  | Imm16_t : type
-  | Target26_t : type
-  | Instruction_t : type
-  | Pair_t (t1 t2: type) : type
-  | Unit_t : type
-.
+  Require Import Shared.Bits.
 
-  Definition tipe := type.
-  Definition tipe_eq : forall (t1 t2:tipe), {t1=t2} + {t1<>t2}.
-    intros ; decide equality.
-  Defined.
-
-  Definition int5 := Word.int 4.
-  Definition int26 := Word.int 25.
-
-  Fixpoint tipe_m (t:tipe) := 
-    match t with 
-      | Int_t => Z
-      | Register_t => register
-      | Shamt5_t => int5
-      | Imm16_t => int16
-      | Target26_t => int26
-      | Instruction_t => instr
-      | Pair_t t1 t2 => ((tipe_m t1) * (tipe_m t2))%type
-      | Unit_t => unit
-    end.
-End MIPS_PARSER_ARG.
-
-
-Module MIPS_PARSER.
-  Module MIPS_BASE_PARSER := Parser.Parser(MIPS_PARSER_ARG).
-  Require Import MIPSSyntax.
-  Require Import Bits.
+  Require Import MIPSModel.ParserArg.
+  Require Import MIPSModel.Parser.
   Import MIPS_PARSER_ARG.
-  Import MIPS_BASE_PARSER.
 
-  Definition int_t := tipe_t Int_t.
-  Definition register_t := tipe_t Register_t.
-  Definition instruction_t := tipe_t Instruction_t.
-  Definition shamt5_t := tipe_t Shamt5_t.
-  Definition imm16_t := tipe_t Imm16_t.
-  Definition target26_t := tipe_t Target26_t.
-  Definition myunit_t := tipe_t Unit_t.
+  Definition int_t := User_t Int_t.
+  Definition register_t := User_t Register_t.
+  Definition instruction_t := User_t Instruction_t.
+  Definition shamt5_t := User_t Shamt5_t.
+  Definition imm16_t := User_t Imm16_t.
+  Definition target26_t := User_t Target26_t.
 
   (* combinators for building parsers *)
-  Definition bit(x:bool) : parser char_t := Char_p x.
-  Definition never t : parser t := Zero_p t.
-  Definition always t (x:result_m t) : parser t := @Map_p unit_t t (fun (_:unit) => x) Eps_p.
-  Definition alt t (p1 p2:parser t) : parser t := Alt_p p1 p2.
-  Definition alts t (ps: list (parser t)) : parser t := List.fold_right (@alt t) (@never t) ps.
-  Definition map t1 t2 (p:parser t1) (f:result_m t1 -> result_m t2) : parser t2 := 
-    @Map_p t1 t2 f p.
+  Definition bit(x:bool) : grammar Char_t := Char x.
+  Definition never t : grammar t := Zero t.
+  Definition always t (x:interp t) : grammar t := @Map Unit_t t (fun (_:unit) => x) Eps.
+  Definition alt t (p1 p2:grammar t) : grammar t := 
+    Map _ (fun (x:interp (Sum_t t t)) => match x with inl a => a | inr b => b end) 
+        (Alt p1 p2).
+
+  Fixpoint alts0 t (ps:list (grammar t)) : grammar t := 
+    match ps with 
+      | nil => @never t
+      | p::nil => p
+      | p::rest => alt p (alts0 rest)
+    end.
+
+  Fixpoint half A (xs ys zs: list A) : (list A) * (list A) := 
+    match xs with 
+      | nil => (ys,zs) 
+      | h::t => half t zs (h::ys)
+    end.
+
+  Fixpoint alts' n t (ps:list (grammar t)) : grammar t := 
+    match n, ps with 
+      | 0%nat, _ => alts0 ps
+      | S n, nil => @never t
+      | S n, p::nil => p
+      | S n, ps => 
+        let (ps1,ps2) := half ps nil nil in 
+          let g1 := alts' n ps1 in 
+            let g2 := alts' n ps2 in 
+              alt g1 g2
+    end.
+
+  Definition alts t (ps:list (grammar t)) : grammar t := alts' 20 ps.
+  Definition map t1 t2 (p:grammar t1) (f:interp t1 -> interp t2) : grammar t2 := 
+    @Map t1 t2 f p.
   Implicit Arguments map [t1 t2].
-  Definition seq t1 t2 (p1:parser t1) (p2:parser t2) : parser (pair_t t1 t2) := Cat_p p1 p2.
-  Definition cons t (pair : result_m (pair_t t (list_t t))) : result_m (list_t t) := 
+  Definition seq t1 t2 (p1:grammar t1) (p2:grammar t2) : grammar (Pair_t t1 t2) := Cat p1 p2.
+  Definition cons t (pair : interp (Pair_t t (List_t t))) : interp (List_t t) := 
     (fst pair)::(snd pair).
-  Definition seqs t (ps:list (parser t)) : parser (list_t t) := 
+  Definition seqs t (ps:list (grammar t)) : grammar (List_t t) := 
     List.fold_right (fun p1 p2 => map (seq p1 p2) (@cons t)) 
-      (@always (list_t t) (@nil (result_m t))) ps.
+      (@always (List_t t) (@nil (interp t))) ps.
 
   (*Useful bit and string manipulators*)
   Fixpoint string_to_bool_list (s:string) : list bool := 
@@ -109,27 +97,27 @@ Module MIPS_PARSER.
         (if ascii_dec a "0"%char then false else true)::(string_to_bool_list s)
     end.
 
-  Fixpoint bits_n (n:nat) : result := 
+  Fixpoint bits_n (n:nat) : type := 
     match n with 
-      | 0%nat => unit_t
-      | S n => pair_t char_t (bits_n n)
+      | 0%nat => Unit_t
+      | S n => Pair_t Char_t (bits_n n)
     end.
-  Fixpoint field'(n:nat) : parser (bits_n n) := 
+  Fixpoint field'(n:nat) : grammar (bits_n n) := 
     match n with 
-      | 0%nat => Eps_p
-      | S n => Cat_p Any_p (field' n)
+      | 0%nat => Eps
+      | S n => Cat Any (field' n)
     end.
-  Fixpoint bits2Z(n:nat)(a:Z) : result_m (bits_n n) -> result_m int_t := 
+  Fixpoint bits2Z(n:nat)(a:Z) : interp (bits_n n) -> interp int_t := 
     match n with 
       | 0%nat => fun _ => a
       | S n => fun p => bits2Z n (2*a + (if (fst p) then 1 else 0)) (snd p)
     end.
-  Definition bits2int(n:nat)(bs:result_m (bits_n n)) : result_m int_t := bits2Z n 0 bs.
-  Fixpoint bits (x:string) : parser (bits_n (String.length x)) := 
+  Definition bits2int(n:nat)(bs:interp (bits_n n)) : interp int_t := bits2Z n 0 bs.
+  Fixpoint bits (x:string) : grammar (bits_n (String.length x)) := 
     match x with 
-      | EmptyString => Eps_p
+      | EmptyString => Eps
       | String c s => 
-        (Cat_p (Char_p (if ascii_dec c "0"%char then false else true)) (bits s))
+        (Cat (Char (if ascii_dec c "0"%char then false else true)) (bits s))
     end.
   Fixpoint string2int' (s:string) (a:Z) : Z :=
     match s with
@@ -140,64 +128,63 @@ Module MIPS_PARSER.
   Definition string2int (s:string) : Z :=
     string2int' s 0.
 
-
   (* notation for building parsers *)
   Infix "|+|" := alt (right associativity, at level 80).
   Infix "$" := seq (right associativity, at level 70).
   Infix "@" := map (right associativity, at level 75).
-  Notation "e %% t" := (e : result_m t) (at level 80).
-  Definition bitsleft t (s:string)(p:parser t) : parser t := 
+  Notation "e %% t" := (e : interp t) (at level 80).
+  Definition bitsleft t (s:string)(p:grammar t) : grammar t := 
     bits s $ p @ (@snd _ _).
   Infix "$$" := bitsleft (right associativity, at level 70).
 
-  Definition anybit : parser char_t := Any_p.
+  Definition anybit : grammar Char_t := Any.
   Definition field(n:nat) := (field' n) @ (bits2int n).
-  Definition reg := (field 5) @ ((fun z => Reg (Zabs_nat z)) : _ -> result_m register_t).
-  Definition imm_p := (field 16) @ (@Word.repr 15 : _ -> result_m imm16_t).
-  Definition target_p := (field 26) @ (@Word.repr 25 : _ -> result_m target26_t).
-  Definition shamt_p := (field 5) @ (@Word.repr 4 : _ -> result_m shamt5_t).
+  Definition reg := (field 5) @ ((fun z => Reg (Zabs_nat z)) : _ -> interp register_t).
+  Definition imm_p := (field 16) @ (@Word.repr 15 : _ -> interp imm16_t).
+  Definition target_p := (field 26) @ (@Word.repr 25 : _ -> interp target26_t).
+  Definition shamt_p := (field 5) @ (@Word.repr 4 : _ -> interp shamt5_t).
  
-  Definition creg_p (s:string) : parser register_t :=
+  Definition creg_p (s:string) : grammar register_t :=
     ((bits s)@(fun _ => Reg (Zabs_nat (string2int s)) %% register_t)).
-  Definition reg0_p : parser register_t :=
+  Definition reg0_p : grammar register_t :=
     creg_p "00000".
-  Definition cshamt_p (s:string) : parser shamt5_t :=
+  Definition cshamt_p (s:string) : grammar shamt5_t :=
     let sfval := @Word.repr 4 (string2int s) in
     ((bits s)@(fun _ => sfval %% shamt5_t)).
-  Definition shamt0_p : parser shamt5_t :=
+  Definition shamt0_p : grammar shamt5_t :=
     cshamt_p "00000".
-  Definition cfcode_p (s:string) : parser myunit_t :=
-    ((bits s)@(fun _ => tt %%myunit_t)).
+  Definition cfcode_p (s:string) : grammar Unit_t :=
+    ((bits s)@(fun _ => tt %%Unit_t)).
 
   (*Generic Instruction Format Parsers*)
-  Definition i_p_gen (opcode: string) (rs_p : parser register_t) (rt_p : parser register_t) 
-    (immf_p : parser imm16_t) (InstCon : ioperand -> instr):=
+  Definition i_p_gen (opcode: string) (rs_p : grammar register_t) (rt_p : grammar register_t) 
+    (immf_p : grammar imm16_t) (InstCon : ioperand -> instr):=
     opcode $$ rs_p $ rt_p $ immf_p @
     (fun p =>
       match p with
         | (r1,(r2,immval)) => InstCon (Iop r1 r2 immval)
       end %% instruction_t).
-  Definition i_p (opcode: string) (InstCon : ioperand -> instr) : parser instruction_t :=
+  Definition i_p (opcode: string) (InstCon : ioperand -> instr) : grammar instruction_t :=
     i_p_gen opcode reg reg imm_p InstCon.
-  Definition j_p_gen (opcode: string) (targetf_p : parser target26_t) (InstCon : joperand -> instr) 
-    : parser instruction_t :=
+  Definition j_p_gen (opcode: string) (targetf_p : grammar target26_t) (InstCon : joperand -> instr) 
+    : grammar instruction_t :=
     opcode $$ targetf_p @
     (fun tval => InstCon (Jop tval) %% instruction_t).
-  Definition j_p (opcode: string) (InstCon: joperand -> instr) : parser instruction_t :=
+  Definition j_p (opcode: string) (InstCon: joperand -> instr) : grammar instruction_t :=
     j_p_gen opcode target_p InstCon.
-  Definition r_p_gen (opcode: string) (rs_p: parser register_t) (rt_p: parser register_t)
-    (rd_p: parser register_t) (shamtf_p: parser shamt5_t) (fcode_p: parser myunit_t) (InstCon: roperand ->instr):=
+  Definition r_p_gen (opcode: string) (rs_p: grammar register_t) (rt_p: grammar register_t)
+    (rd_p: grammar register_t) (shamtf_p: grammar shamt5_t) (fcode_p: grammar Unit_t) (InstCon: roperand ->instr):=
     opcode $$ rs_p $ rt_p $ rd_p $ shamtf_p $ fcode_p @
     (fun p =>
       match p with
         | (r1,(r2,(r3,(shval,_)))) => InstCon (Rop r1 r2 r3 shval) %% instruction_t
       end).
-  Definition r_p (opcode: string) (fcode: string) (InstCon: roperand -> instr) : parser instruction_t :=
-    r_p_gen opcode reg reg reg shamt_p ((bits fcode)@(fun _ => tt %%myunit_t)) InstCon. 
+  Definition r_p (opcode: string) (fcode: string) (InstCon: roperand -> instr) : grammar instruction_t :=
+    r_p_gen opcode reg reg reg shamt_p ((bits fcode)@(fun _ => tt %%Unit_t)) InstCon. 
   Definition r_p_zsf (opcode: string) (fcode: string) (InstCon: roperand -> instr)
-    : parser instruction_t :=
+    : grammar instruction_t :=
     r_p_gen opcode reg reg reg shamt0_p (cfcode_p fcode) InstCon.
-  Definition shift_p (fcode: string) (InstCon: roperand -> instr) : parser instruction_t :=
+  Definition shift_p (fcode: string) (InstCon: roperand -> instr) : grammar instruction_t :=
     r_p_gen "000000" reg0_p reg reg shamt_p (cfcode_p fcode) InstCon.
 
   (*Specific Instruction Parsers*)
@@ -256,8 +243,8 @@ Module MIPS_PARSER.
   Definition XORI_p := i_p "001110" XORI.
 
   
-  (*Large parser list*)
-  Definition instr_parser_list : list (parser instruction_t) := 
+  (*Large grammar list*)
+  Definition instr_grammar_list : list (grammar instruction_t) := 
     ADD_p :: ADDI_p :: ADDIU_p :: ADDU_p ::
     AND_p :: ANDI_p :: BEQ_p :: BGEZ_p :: BGEZAL_p ::
     BGTZ_p :: BLEZ_p :: BLTZ_p :: BLTZAL_p ::
@@ -269,11 +256,20 @@ Module MIPS_PARSER.
     SRL_p :: SRLV_p :: SUB_p :: SUBU_p :: SW_p :: XOR_p :: XORI_p ::
     nil.
 
-  Definition instr_parser : parser instruction_t :=
-    alts instr_parser_list.
-  Definition instr_regexp_pair := parser2regexp instr_parser.
-  Definition instr_regexp := fst instr_regexp_pair.
-  Definition instr_regexp_ctxt := snd instr_regexp_pair.
+  Definition instr_grammar : grammar instruction_t :=
+    alts instr_grammar_list.
+  Definition instr_regexp := projT1 (split_grammar instr_grammar).
+
+  Definition parse_string (s: string) : list instr :=
+    let cs := string_to_bool_list s in
+    naive_parse instr_grammar cs.
+
+  Definition test1 := 
+    match (parse_string "00001000000000000000000000000000") with
+      | (J jop)::tl => 1
+      | _ => 0
+    end.
+  (* Eval compute in test1. *)
 
   Definition word_explode (b:int32) : list bool :=
   let bs := Word.bits_of_Z 32 (Word.unsigned b) in
@@ -284,24 +280,8 @@ Module MIPS_PARSER.
       end
     ) 32%nat.
 
-  Definition parse_string (s: string) : list instr :=
-    let cs := string_to_bool_list s in
-    let r' := deriv_parse' instr_regexp cs in
-    let wf' := wf_derivs instr_regexp_ctxt cs instr_regexp 
-      (p2r_wf instr_parser _) in
-    apply_null (instr_regexp_ctxt) r' wf'.
-
-  Definition test1 := 
-    match (parse_string "00001000000000000000000000000000") with
-      | (J jop)::tl => 1
-      | _ => 0
-    end.
-
   Definition parse_word (w:int32) : list instr :=
     let cs := word_explode w in
-    let r' := deriv_parse' instr_regexp cs in
-    let wf' := wf_derivs instr_regexp_ctxt cs instr_regexp 
-      (p2r_wf instr_parser _) in
-    apply_null (instr_regexp_ctxt) r' wf'.
+    naive_parse instr_grammar cs.
   
-End MIPS_PARSER.
+(* End MIPS_PARSER. *)
