MIPSmodel/Regexp.v
@@ -1,0 +1,296 @@
+Require Import Coq.Structures.OrdersAlt.
+Require Import CommonTacs.
+Require Import Xform.
+Require Import ParserArg.
+Import MIPS_PARSER_ARG.
+
+Set Implicit Arguments.
+
+Inductive regexp : Set := 
+| rEps : regexp
+| rZero : regexp
+| rChar : char_p -> regexp
+| rAny : regexp
+| rCat : regexp -> regexp -> regexp
+| rAlt : regexp -> regexp -> regexp
+| rStar : regexp -> regexp.
+
+(** Compute the return [xtype] of an [regexp]. *)
+Fixpoint regexp_type (pg : regexp) : xtype := 
+  match pg with 
+    | rEps => xUnit_t
+    | rZero => xVoid_t
+    | rChar _ => xChar_t
+    | rAny => xChar_t
+    | rCat pg1 pg2 => xPair_t (regexp_type pg1) (regexp_type pg2)
+    | rAlt pg1 pg2 => xSum_t (regexp_type pg1) (regexp_type pg2)
+    | rStar pg => xList_t (regexp_type pg)
+  end.
+
+Inductive in_regexp : forall a, list char_p -> xt_interp (regexp_type a) -> Prop :=
+| InrEps : forall s v, s = nil -> v = tt -> in_regexp rEps s v
+| InrChar : forall c s v, s = c::nil -> v = c -> in_regexp (rChar c) s v
+| InrAny : forall c s v, s = c::nil -> v = c -> in_regexp rAny s v
+| InrCat : 
+    forall a1 a2 s1 s2 v1 v2 s v,
+      in_regexp a1 s1 v1 -> in_regexp a2 s2 v2 -> s = s1 ++ s2 -> v = (v1,v2) -> 
+      in_regexp (rCat a1 a2) s v
+| InrAlt_l : 
+    forall a1 a2 s v1 v, 
+      in_regexp a1 s v1 -> v = inl _ v1 -> in_regexp (rAlt a1 a2) s v
+| InrAlt_r : 
+    forall a1 a2 s v2 v, 
+      in_regexp a2 s v2 -> v = inr _ v2 -> in_regexp (rAlt a1 a2) s v
+| InrStar_eps : forall a s v, s = nil -> v = nil -> in_regexp (rStar a) s v
+| InrStar_cons : 
+    forall a s1 v1 s2 v2 s v,
+      in_regexp a s1 v1 -> in_regexp (rStar a) s2 v2 -> 
+      s1 <> nil -> s = s1 ++ s2 -> v = v1::v2 -> in_regexp (rStar a) s v.
+Hint Constructors in_regexp.
+
+(** * Inversion principles for [regexp]s. *)
+
+Lemma inv_eps : forall s v, in_regexp rEps s v -> s = nil /\ v = tt.
+Proof. intros. inversion H. crush. Qed.
+
+Lemma inv_zero : forall s v, in_regexp rZero s v -> False.
+Proof. intros. inversion H. Qed.
+
+Lemma inv_char : forall c s v, in_regexp (rChar c) s v -> s = c::nil /\ v = c.
+Proof.  intros. inversion H. subst. crush. Qed.
+
+Lemma inv_any : forall s v, in_regexp rAny s v -> s = v::nil.
+Proof.  intros. inversion H. crush. Qed.
+
+Lemma inv_cat : forall r1 r2 s v, in_regexp (rCat r1 r2) s v -> 
+  exists s1, exists s2, exists v1, exists v2, 
+    in_regexp r1 s1 v1 /\ in_regexp r2 s2 v2 /\ s = s1++s2 /\ v = (v1,v2).
+Proof.
+  intros ; inversion H ; subst ; crush. exists s1. exists s2. exists v1. exists v2.
+  auto.
+Qed.
+
+Lemma inv_cat_nil : forall r1 r2 v, in_regexp (rCat r1 r2) nil v -> 
+  exists v1, exists v2, in_regexp r1 nil v1 /\ in_regexp r2 nil v2 /\ v = (v1,v2).
+Proof. intros. apply inv_cat in H.
+  destruct H as [s1 [s2 [v1 [v2 H1]]]].
+  sim. exists v1, v2.
+  symmetry in H1. apply app_eq_nil in H1.
+  crush.
+Qed.
+
+Lemma inv_alt : forall r1 r2 s v, in_regexp (rAlt r1 r2) s v -> 
+  (exists v1, in_regexp r1 s v1 /\ v = inl _ v1) \/
+  (exists v2, in_regexp r2 s v2 /\ v = inr _ v2) .
+Proof. intros ; inversion H ; subst ; crush. Qed.
+
+Lemma inv_star: forall r s v, in_regexp (rStar r) s v -> 
+  (s = nil /\ v = nil) \/
+  (exists s1 s2 v1 v2, 
+     in_regexp r s1 v1 /\ in_regexp (rStar r) s2 v2 /\
+     s1 <> nil /\ s = s1++s2 /\ v=v1::v2).
+Proof. intros. inversion H; try crush. 
+  right. exists s1, s2, v1, v2. crush.
+Qed.
+
+Lemma inv_star_nil: forall r v, in_regexp (rStar r) nil v -> v = nil.
+Proof. intros. apply inv_star in H.
+  destruct H. crush.
+  sim. destruct x; crush.
+Qed.
+
+(** Inversion tactic for [regexp]. *)
+Ltac in_regexp_inv := 
+  match goal with 
+    | [ H: in_regexp rZero _ _ |- _ ] => contradiction (inv_zero H)
+    | [ H : in_regexp rEps _ _ |- _ ] => 
+      generalize (inv_eps H) ; clear H ; crush
+    | [ H : in_regexp (rChar _) _ _ |- _] => 
+      generalize (inv_char H) ; clear H ; crush
+    | [ H : in_regexp rAny _ _ |- _] => 
+      generalize (inv_any H) ; clear H ; crush
+    | [ H : in_regexp (rCat _ _) nil _ |- _] => 
+      generalize (inv_cat_nil H) ; clear H ; crush
+    | [ H : in_regexp (rCat _ _) _ _ |- _] => 
+      generalize (inv_cat H) ; clear H ; crush
+    | [ H : in_regexp (rAlt _ _) _ _ |- _] => 
+      generalize (inv_alt H) ; clear H ;  crush
+    | [ H : in_regexp (rStar _) nil _ |- _] => 
+      generalize (inv_star_nil H) ; clear H ;  crush
+    | [ H : in_regexp (rStar _) _ _ |- _] => 
+      generalize (inv_star H) ; clear H ;  crush
+  end.
+
+(** This function computes the list of all values v, such that 
+    [in_regexp nil v] holds. *)
+Fixpoint regexp_extract_nil (r:regexp) : list (xt_interp (regexp_type r)) := 
+  match r return list (xt_interp (regexp_type r)) with
+    | rEps => tt::nil
+    | rZero => nil
+    | rChar _ => nil
+    | rAny => nil
+    | rCat ag1 ag2 => list_prod (regexp_extract_nil ag1) (regexp_extract_nil ag2)
+    | rAlt ag1 ag2 => 
+      (List.map (fun x => inl _ x) (regexp_extract_nil ag1)) ++ 
+      (List.map (fun x => inr _ x) (regexp_extract_nil ag2))
+    | rStar ag => nil::nil
+  end.
+
+(** Nullable (r) returns true iff r can match the empty string *)
+Fixpoint regexp_nullable (r:regexp) : bool :=
+  match r with
+    | rZero | rChar _ | rAny => false
+    | rEps => true
+    | rCat r1 r2 => regexp_nullable r1 && regexp_nullable r2
+    | rAlt r1 r2 => regexp_nullable r1 || regexp_nullable r2
+    | rStar r1 => true
+  end.
+
+Fixpoint regexp_always_rejects (r:regexp) : bool :=
+  match r with
+    | rEps => false
+    | rChar _ => false
+    | rAny => false
+    | rZero => true
+    | rAlt r1 r2 => regexp_always_rejects r1 && regexp_always_rejects r2
+    | rCat r1 r2 => regexp_always_rejects r1 || regexp_always_rejects r2
+    | rStar _ => false
+  end.
+
+(** * Ordering for regexps *)
+
+(** Use lexicographic ordering when ordering two regexps. *)
+Fixpoint compare_re (r1 r2:regexp) : comparison := 
+  match r1 with
+    | rEps => match r2 with
+                | rEps => Eq
+                | _ => Lt
+              end
+    | rZero => match r2 with
+                 | rEps => Gt
+                 | rZero => Eq
+                 | _ => Lt
+               end
+    | rChar c1 => 
+      match r2 with
+        | rEps | rZero => Gt
+        | rChar c2 => char_cmp c1 c2
+        | _ => Lt
+      end
+    | rAny => match r2 with
+                | rEps | rZero | rChar _ => Gt
+                | rAny => Eq
+                | _ => Lt
+              end
+    | rCat r11 r12 =>
+      match r2 with
+        | rEps | rZero | rChar _ | rAny => Gt
+        | rCat r21 r22 =>
+          let cp := compare_re r11 r21 in
+          match cp with
+            | Eq => compare_re r12 r22
+            | _ => cp
+          end
+        | _ => Lt
+      end
+    | rAlt r11 r12 =>
+      match r2 with
+        | rEps | rZero | rChar _ | rAny | rCat _ _ => Gt
+        | rAlt r21 r22 =>
+          let cp := compare_re r11 r21 in
+          match cp with
+            | Eq => compare_re r12 r22
+            | _ => cp
+          end
+        | _ => Lt
+      end
+    | rStar r11 => 
+      match r2 with
+        | rEps | rZero | rChar _ | rAny | rCat _ _ | rAlt _ _ => Gt
+        | rStar r21 => compare_re r11 r21
+      end
+  end.
+
+Lemma compare_re_eq_leibniz: 
+  forall r1 r2, compare_re r1 r2 = Eq -> r1 = r2.
+Proof. induction r1; try (destruct r2; simpl; congruence; fail). 
+       Case "rChar".
+       destruct r2; simpl; try congruence. intros.
+       rewrite (char_eq_leibniz c c0) ; auto.
+       Case "rCat".
+       destruct r2; simpl; try congruence.
+       remember_rev (compare_re r1_1 r2_1) as cmp.
+       destruct cmp; crush_hyp.
+       Case "rAlt".
+       destruct r2; simpl; try congruence.
+       remember_rev (compare_re r1_1 r2_1) as cmp.
+       destruct cmp; crush_hyp.
+       Case "rStar".
+       destruct r2; simpl; try congruence.
+       crush_hyp.
+Qed.
+
+Module REOrderedTypeAlt <: OrderedTypeAlt.
+  Definition t:=regexp.
+  Definition compare := compare_re.
+
+  Lemma compare_sym : forall r1 r2, compare r2 r1 = CompOpp (compare r1 r2).
+  Proof. induction r1; try (destruct r2; trivial; fail).
+    Case "rChar".
+      destruct r2; trivial. 
+      generalize (CharOrderedTypeAlt.compare_sym c c0). simpl. auto.
+    Case "rCat".
+      destruct r2; trivial. simpl.
+        rewrite (IHr1_1 r2_1). destruct (compare r1_1 r2_1); simpl; eauto.
+    Case "rAlt".
+      destruct r2; trivial. simpl.
+        rewrite (IHr1_1 r2_1). destruct (compare r1_1 r2_1); simpl; eauto.
+    Case "rStar".
+      destruct r2; trivial. simpl. eauto.
+  Qed.
+
+  Lemma compare_trans:
+    forall cmp r1 r2 r3,
+      compare r1 r2 = cmp -> compare r2 r3 = cmp -> compare r1 r3 = cmp.
+  Proof. intros cmp r1. generalize cmp.
+    induction r1;
+    try (destruct r2; destruct r3; simpl; congruence; fail).
+    Local Ltac trans_simp :=
+      match goal with
+        | [H:compare ?R1 ?R2 = Eq |- _] => 
+          apply compare_re_eq_leibniz in H; subst R2
+      end.
+    Case "rChar".
+      destruct r2; destruct r3; simpl; try congruence.
+      apply (CharOrderedTypeAlt.compare_trans).
+    Case "rCat".
+      destruct r2; destruct r3; simpl; try congruence.
+      remember_rev (compare r1_1 r2_1) as cmp1.
+      remember_rev (compare r2_1 r3_1) as cmp2.
+      destruct cmp1; destruct cmp2; 
+        try (repeat trans_simp; crush; fail).
+        assert (H10:compare r1_1 r3_1 = Eq) by eauto.
+        rewrite H10. eauto.
+        assert (H10:compare r1_1 r3_1 = Lt) by eauto.
+        rewrite H10. eauto.
+        assert (H10:compare r1_1 r3_1 = Gt) by eauto.
+        rewrite H10. eauto.
+    Case "rAlt".
+      destruct r2; destruct r3; simpl; try congruence.
+      remember_rev (compare r1_1 r2_1) as cmp1.
+      remember_rev (compare r2_1 r3_1) as cmp2.
+      destruct cmp1; destruct cmp2; 
+        try (repeat trans_simp; crush; fail).
+        assert (H10:compare r1_1 r3_1 = Eq) by eauto.
+        rewrite H10. eauto.
+        assert (H10:compare r1_1 r3_1 = Lt) by eauto.
+        rewrite H10. eauto.
+        assert (H10:compare r1_1 r3_1 = Gt) by eauto.
+        rewrite H10. eauto.
+    Case "rStar".  
+      destruct r2; destruct r3; simpl; (congruence || eauto).
+  Qed.
+
+End REOrderedTypeAlt.
+
+Module REOrderedType := OT_from_Alt REOrderedTypeAlt.
